10/17 update

src/basicmodal/semantics/completeness.lean
@@ -12,13 +12,23 @@ def canonical (AX : ctx) [hax : sem_cons AX] : frame :=
   rel := λ xΓ yΔ, ∀ φ : form, □φ ∈ xΓ.val → φ ∈ yΔ.val
 }
 
+--instance : sem_cons T_axioms := sem_consT
+def T_canonical : frame := @canonical T_axioms sem_consT
+
+--instance : sem_cons S4_axioms := sem_consS4
+def S4_canonical : frame := @canonical S4_axioms sem_consS4
+
+-- instance : sem_cons S5_axioms := sem_consS5
+def S5_canonical : frame := @canonical S5_axioms sem_consS5
+
 def val_canonical (AX : ctx) [hax : sem_cons AX] : nat → (canonical AX).states → Prop :=
   λ n, λ xΓ : (canonical AX).states, (p n) ∈ xΓ.val
 
 lemma existence (AX : ctx) (hax : sem_cons AX) (xΓ : (canonical AX).states) :
-  ∀ φ, ◇φ ∈ xΓ.val → ∃ yΔ : (canonical AX).states, φ ∈ yΔ.val ∧ (canonical AX).rel xΓ yΔ :=
+  ∀ φ, ◇φ ∈ xΓ.val ↔ ∃ yΔ : (canonical AX).states, φ ∈ yΔ.val ∧ (canonical AX).rel xΓ yΔ :=
 begin
-intros φ h1,
+intro φ, split,
+intro h1,
 let Γbox : ctx := {ψ : form | □ψ ∈ xΓ.val},
 have h1 : ax_consist AX (Γbox ∪ {φ}), 
 {by_contradiction h2, simp at h2,
@@ -44,7 +54,17 @@ have h5 := set.union_subset_iff.mp h3,
 cases h5, split, simp at h5_right, exact h5_right,
 have h3 : ∀ φ : form, □φ ∈ xΓ.val → φ ∈ xΔ.val,
 intros ψ h4, apply h5_left, exact h4,
-exact h3
+exact h3,
+simp at *,
+intros yΔ h1 h2,
+have h3 := h2 φ, 
+by_contradiction h4,
+have h5 := (max_notiff AX xΓ.1 xΓ.2 (◇φ)).mp h4,
+have h6 := (max_dn AX xΓ.1 xΓ.2 (□¬φ)).mpr h5,
+have h7 := h2 (¬φ), specialize h7 h6,
+simp at *,
+have h8 := (max_notiff AX yΔ.1 yΔ.2 φ).mpr h7,
+exact absurd h1 h8
 end
 
 lemma truth (AX : ctx) (hax : sem_cons AX) (xΓ : (canonical AX).states) : 
@@ -88,7 +108,7 @@ split, intros h1,
 by_contradiction h2,
 have h4 : ◇(¬φ) ∈ xΓ.val → ∃ yΔ : (canonical AX).states, 
   (¬φ) ∈ yΔ.val ∧ (canonical AX).rel xΓ yΔ,
-from existence AX hax xΓ (¬φ),
+from (existence AX hax xΓ (¬φ)).mp,
 have h5 := max_boxdn AX xΓ.1 xΓ.2 φ ((max_notiff AX xΓ.1 xΓ.2 φ.box).mp h2),
 simp at *,
 specialize h4 h5, cases h4 with xΔ h4, cases h4 with h4 h6,
@@ -120,6 +140,18 @@ exact h3,
 exact h6
 end 
 
+theorem forcesAX (AX : ctx) (hax : sem_cons AX) : 
+  forces_ctx (canonical AX) (val_canonical AX) AX :=
+begin
+rw forces_ctx,
+intros φ xΓ h1,
+have h2 : prfK AX ((¬⊥) ⊃ φ), from mp pl1 (ax h1),
+have h3 : ∀ ψ ∈ list.nil, ψ ∈ xΓ.val, 
+{intros ψ h3, have h5 := list.ne_nil_of_length_pos (list.length_pos_of_mem h3),
+simp at *, exact false.elim h5},
+have h4 : φ ∈ xΓ.val, from exercise1 xΓ.2 h3 h2,
+exact (truth AX hax xΓ φ).mpr h4
+end
 
 theorem completeness (AX : ctx) (hax : sem_cons AX) (φ : form) : 
   global_sem_csq AX φ → prfK AX φ :=
@@ -127,15 +159,15 @@ begin
 rw ←not_imp_not, intro h1,
 have h2 : ax_consist AX {¬φ}, from comphelper AX φ hax h1,
 have h3 : ∃ Γ', max_ax_consist AX Γ' ∧ {¬φ} ⊆ Γ', from lindenbaum AX {¬φ} h2,
-cases h3 with Γ' h3, cases h3 with h3 h4, simp at *,
+simp at *,
+cases h3 with Γ' h3, cases h3 with h3 h4, 
 rw global_sem_csq, 
 push_neg,
 let f := canonical, use f AX,
 let v := val_canonical, use v AX,
 let xΓ' : (f AX).states := ⟨Γ', h3⟩, use xΓ',
-split, rw forces_ctx,
-intros ψ y h5, 
-sorry,
+split, 
+exact forcesAX AX hax,
 have h5 : forces (f AX) (v AX) xΓ' (¬φ) ↔ ((¬φ) ∈ xΓ'.val), 
   from truth AX hax xΓ' ¬φ,
 cases h5 with h5 h6,
@@ -144,48 +176,169 @@ have h7 : ¬forces (f AX) (v AX) xΓ' φ ↔ forces (f AX) (v AX) xΓ' ¬φ,
 cases h7 with h7 h8, apply h8, apply h6, simp at *, exact h4
 end
 
+-- if φ is not a global semantic consequence of AX, 
+-- then ∃ xΓ ∈ canonical model, such that ¬ forces (canonical ax) (val canonical ax) xΓ φ
+lemma renameme (AX : ctx) (φ : form) (hax : sem_cons AX) : (¬ global_sem_csq AX φ) → 
+  ∃ xΓ : (canonical AX).states, ¬ forces (canonical AX) (val_canonical AX) xΓ φ :=
+begin
+  intro h1,
+  have h2 : forces_ctx (canonical AX) (val_canonical AX) AX, from forcesAX AX hax,
+  rw forces_ctx at h2, specialize h2 φ, sorry
+end
+
+lemma T_reflexive : T_canonical ∈ ref_class :=
+begin
+rw ref_class, rw set.mem_set_of_eq, rw reflexive,
+intros x φ h1,
+have h2 : (∀ ψ ∈ [□φ], ψ ∈ x.1) → prfK T_axioms (fin_conj [□φ] ⊃ φ) → φ ∈ x.1, 
+  from exercise1 x.2, simp at *,
+have h3 : prfK T_axioms (fin_conj [φ.box] ⊃ φ), 
+{repeat {rw fin_conj},
+have h4 : prfK T_axioms (φ.box ⊃ φ), 
+{refine ax _, rw T_axioms, simp},
+exact cut (mp pl5 phi_and_true) h4},
+exact h2 h1 h3
+end
 
 theorem T_completeness (φ : form) : F_valid φ ref_class → prfK T_axioms φ :=
 begin
-intros h1,
-have h2 : global_sem_csq T_axioms φ → prfK T_axioms φ, 
+rw ←not_imp_not, intro h1,
+have h2 : ax_consist T_axioms {¬φ}, from comphelper T_axioms φ sem_consT h1,
+simp at *,
+have h3 : ∃ Γ', max_ax_consist T_axioms Γ' ∧ {¬φ} ⊆ Γ', 
+  from lindenbaum T_axioms {¬φ} h2,
+cases h3 with Γ' h3, cases h3 with h3 h4, simp at *,
+rw F_valid, push_neg,
+let f := T_canonical, use f,
+split, exact T_reflexive,
+let v := val_canonical, use (@v T_axioms sem_consT),
+have h5 : (¬ global_sem_csq T_axioms φ) → 
+  ∃ xΓ : f.states, ¬ forces f (@val_canonical T_axioms sem_consT) xΓ φ, 
+  from renameme T_axioms φ sem_consT,
+have h6 : global_sem_csq T_axioms φ → prfK T_axioms φ, 
   from completeness T_axioms sem_consT φ,
-apply h2, clear h2,
-rw global_sem_csq, intros f v x h3,
-rw F_valid at h1,
-apply h1, 
-sorry
+rw ←not_imp_not at h6, specialize h6 h1, specialize h5 h6, exact h5
 end
 
+lemma S4_reftrans : S4_canonical ∈ ref_trans_class :=
+begin
+rw ref_trans_class, split,
+rw ref_class, rw set.mem_set_of_eq, rw reflexive,
+intros x φ h1,
+have h2 : (∀ ψ ∈ [□φ], ψ ∈ x.1) → prfK S4_axioms (fin_conj [□φ] ⊃ φ) → φ ∈ x.1, 
+  from exercise1 x.2, simp at *,
+have h3 : prfK S4_axioms (fin_conj [φ.box] ⊃ φ), 
+{repeat {rw fin_conj},
+have h4 : prfK S4_axioms (φ.box ⊃ φ), 
+{refine ax _, rw S4_axioms, simp, rw T_axioms, simp},
+exact cut (mp pl5 phi_and_true) h4},
+exact h2 h1 h3,
+rw trans_class, rw set.mem_set_of_eq, rw transitive,
+intros x y z h1 h2 φ h3, specialize h2 φ, apply h2,
+specialize h1 (□φ), apply h1,
+have h4 : prfK S4_axioms (fin_conj [φ.box] ⊃ φ.box.box), 
+{repeat {rw fin_conj},
+simp at *,
+have h5 : prfK S4_axioms (φ.box ⊃ φ.box.box), 
+{refine ax _, rw S4_axioms, simp},
+exact cut (mp pl5 phi_and_true) h5},
+have h6 : (∀ ψ ∈ [□φ], ψ ∈ x.1) → prfK S4_axioms (fin_conj [□φ] ⊃ φ.box.box) → φ.box.box ∈ x.1, 
+  from exercise1 x.2, simp at *,
+exact h6 h3 h4
+end
 
-theorem S4_completeness (φ : form) : F_valid φ ref_trans_class → prfK S4_axioms φ := sorry
+theorem S4_completeness (φ : form) : F_valid φ ref_trans_class → prfK S4_axioms φ :=
+begin
+rw ←not_imp_not, intro h1,
+have h2 : ax_consist S4_axioms {¬φ}, from comphelper S4_axioms φ sem_consS4 h1,
+simp at *,
+have h3 : ∃ Γ', max_ax_consist S4_axioms Γ' ∧ {¬φ} ⊆ Γ', 
+  from lindenbaum S4_axioms {¬φ} h2,
+cases h3 with Γ' h3, cases h3 with h3 h4, simp at *,
+rw F_valid, push_neg,
+let f := S4_canonical, use f,
+split, exact S4_reftrans,
+let v := val_canonical, use (@v S4_axioms sem_consS4),
+have h5 : (¬ global_sem_csq S4_axioms φ) → 
+  ∃ xΓ : f.states, ¬ forces f (@val_canonical S4_axioms sem_consS4) xΓ φ, 
+  from renameme S4_axioms φ sem_consS4,
+have h6 : global_sem_csq S4_axioms φ → prfK S4_axioms φ, 
+  from completeness S4_axioms sem_consS4 φ,
+rw ←not_imp_not at h6, specialize h6 h1, 
+specialize h5 h6, exact h5
+end
 
-theorem S5_completeness (φ : form) : F_valid φ equiv_class → prfK S5_axioms φ := sorry
+lemma euclid_dual {φ : form} : prfK S5_axioms ((◇(¬φ) ⊃ □(◇(¬φ))) ⊃ (◇(□φ) ⊃ □φ)) :=
+begin
+simp,
+have h1 : prfK S5_axioms (◇(¬φ) ⊃ □(◇¬φ)),
+refine ax _, rw S5_axioms, simp, simp at *,
+have h2 : prfK S5_axioms ((¬□(◇¬φ)) ⊃ ¬(◇¬φ)), from contrapos.mpr h1,
+have h3 : prfK S5_axioms ((¬□(◇¬φ)) ⊃ (□φ)), from cut h2 (mp pl6 dual_equiv1),
+have h4 : prfK S5_axioms ((¬□(◇¬φ)) ↔ (¬¬◇(¬(◇¬φ)))), sorry,
+have h5 : prfK S5_axioms (◇(¬(◇¬φ)) ⊃ (□φ)), from cut dni (cut (mp pl6 h4) h3),
+have h6 : prfK S5_axioms ((◇(□φ)) ⊃ (◇(¬(◇¬φ)))), sorry,
+exact (mp pl1 (cut h6 h5))
+end
+
+lemma S5_equiv : S5_canonical ∈ equiv_class :=
+begin
+rw equiv_ref_euclid,
+split,
+rw ref_class, rw set.mem_set_of_eq,
+rw reflexive,
+intros x φ h1,
+have h2 : (∀ ψ ∈ [□φ], ψ ∈ x.1) → prfK S5_axioms (fin_conj [□φ] ⊃ φ) → φ ∈ x.1, 
+  from exercise1 x.2, simp at *,
+have h3 : prfK S5_axioms (fin_conj [φ.box] ⊃ φ), 
+{repeat {rw fin_conj},
+have h4 : prfK S5_axioms (φ.box ⊃ φ), 
+{refine ax _, rw S5_axioms, simp, rw T_axioms, simp},
+exact cut (mp pl5 phi_and_true) h4},
+exact h2 h1 h3,
+rw euclid_class,
+rw set.mem_set_of_eq,
+rw euclidean,
+intros x y z h1 h2 φ h3,
+specialize h2 φ,
+apply h2, clear h2,
+have h2 : prfK S5_axioms (◇(¬φ) ⊃ □(◇¬φ)), 
+{refine ax _, rw S5_axioms, simp},
+have h4 : prfK S5_axioms (◇(□φ) ⊃ □φ), 
+  from mp euclid_dual h2,
+have h5 : (∀ ψ ∈ [◇(□φ)], ψ ∈ x.1) → 
+  prfK S5_axioms (fin_conj [◇(□φ)] ⊃ □φ) → □φ ∈ x.1, 
+  from exercise1 x.2, simp at *,
+apply h5,
+by_contradiction h6,
+have h7 := (max_notiff S5_axioms x.1 x.2 (¬(¬φ.box).box)).mp h6,
+have h8 := (max_dn S5_axioms x.1 x.2 ((¬φ.box).box)).mpr h7,
+specialize h1 (¬φ.box) h8,
+have h9 := (max_notiff S5_axioms y.1 y.2 (φ.box)).mpr h1,
+simp at *, exact absurd h3 h9,
+exact (cut (mp pl5 phi_and_true) h4)
+end
+
+theorem S5_completeness (φ : form) : F_valid φ equiv_class → prfK S5_axioms φ :=
+begin
+rw ←not_imp_not, intro h1,
+have h2 : ax_consist S5_axioms {¬φ}, from comphelper S5_axioms φ sem_consS5 h1,
+simp at *,
+have h3 : ∃ Γ', max_ax_consist S5_axioms Γ' ∧ {¬φ} ⊆ Γ', 
+  from lindenbaum S5_axioms {¬φ} h2,
+cases h3 with Γ' h3, cases h3 with h3 h4, simp at *,
+rw F_valid, push_neg,
+let f := S5_canonical, use f,
+split, exact S5_equiv,
+let v := val_canonical, use (@v S5_axioms sem_consS5),
+have h5 : (¬ global_sem_csq S5_axioms φ) → 
+  ∃ xΓ : f.states, ¬ forces f (@val_canonical S5_axioms sem_consS5) xΓ φ, 
+  from renameme S5_axioms φ sem_consS5,
+have h6 : global_sem_csq S5_axioms φ → prfK S5_axioms φ, 
+  from completeness S5_axioms sem_consS5 φ,
+rw ←not_imp_not at h6, specialize h6 h1, 
+specialize h5 h6, exact h5
+end
 
 end canonical
 
-
-
-
-
-
-
-
-
-
-
--- lemma completenesshelper {AX : ctx} {φ : form} {C : set (frame)} (hax : sem_cons AX) : 
---   F_valid φ C → (∀ ψ ∈ AX, F_valid ψ C) → prfK AX φ :=
--- begin
--- intros h1 h2,
--- have h3 : global_sem_csq AX φ → prfK AX φ, from completeness AX hax φ,
--- apply h3, clear h3,
--- end
-
--- intros h1,
--- have h2 : (∀ ψ ∈ T_axioms, F_valid ψ ref_class) → prfK T_axioms φ,
--- from completenesshelper sem_consT h1,
--- apply h2, clear h2,
--- intros ψ h2,
--- apply T_helper,
--- exact h2,
